# Prefix sum

### Prefix sum 1D

```cpp
prefix[0] = 0;
for (int i = 1; i <= n; ++i) prefix[i] = prefix[i - 1] + a[i];

sum(i -> j) = prefix[j] - prefix[i - 1];
```

### Prefix sum 2D

```cpp
a[i][0] = 0 ∀ i = 1..m
a[0][i] = 0 ∀ i = 1..n
for (int i = 1; i <= m; ++i)
	for (int j = 1; j <= n; ++j)
		prefix[i][j] = prefix[i - 1][j] + prefix[i][j - 1] 
								 - prefix[i - 1][j - 1]
								 + a[i][j];

sum(x1, x2, y1, y2) = prefix[x2][y2]
										- (prefix[x1 - 1][y2] + prefix[x2][y1 - 1])
										+ prefix[x1 - 1][y1 - 1];
```

### 

### Prefix sum 3D

```cpp
for (int i = 1; i <= m; ++i)
		for (int j = 1; j <= n; ++j)
			for (int k = 1; k <= r; ++k)
				s[i][j][k] = s[i - 1][j][k] + s[i][j - 1][k] + s[i][j][k - 1]
							     - (s[i - 1][j - 1][k] + s[i - 1][j][k - 1] + s[i][j - 1][k - 1])
							     + s[i - 1][j - 1][k - 1] + a[i][j][k];

sum(i1, j1, k1, i2, j2, k2) 
  = s[i2][j2][k2]
  - (s[i1 - 1][j2][k2] + s[i2][j1 - 1][k2] + s[i2][j2][k1 - 1])
	+ (s[i1 - 1][j1 - 1][k2] + s[i1 - 1][j2][k1 - 1] + s[i2][j1 - 1][k1 - 1])
	- s[i1 - 1][j1 - 1][k1 - 1];
```